Towards subject reduction
Proving valid_btys: needs more inversion info on |- tInd args : tau
Add Derive Signature where needed to avoid warnings
Proved inversion lemmas on typing spine
Finished inversion of |- c : mkApps (tInd ind u) args, remain some holes in valid_btys
related to universes and the typing of the branches.

One todo + 2 universes properties

WIP valid_btys

state elim restriction
Backport of cdacc4de201

WIP proving inversion of constructor typing by inductive (provable!)

Finish Construct_Ind_ind_eq

Modify type_local_ctx so that it implies wf_local_env (adding proofs for lets)

Prove a strong subst lemma for typing_spines of it_mkProd_or_LetIn

WIP

Prove substitutivity of `isType (it_mkProd_or_LetIn)`

WIP proving valid_btys

WIP subslet_app_inv proof

WIP rebsing valid_btys and cleaning up

WIP refactoring

Move more defs to the Env and inline them

Fix erasure

Fix proof focusing in PCUIC

Refactor. The remaining safe lemmata all require SR

WIP proving SR for Case

WIP on SR proof

WIP finishing SR proof

WIP proving SR

WIP proving SR for match

Fix after rebase

Force no output of examples due to timing files

Fix after rebase

pcuic/theories/PCUICAstUtils.v
@@ -1,5 +1,5 @@
 From Coq Require Import Ascii String OrderedType Lia Program Arith.
-From MetaCoq.Template Require Import utils.
+From MetaCoq.Template Require Import utils uGraph.
 From MetaCoq.PCUIC Require Import PCUICAst PCUICSize.
 Import List.ListNotations.
 Require Import ssreflect.
@@ -181,6 +181,90 @@ Proof.
   move=> Hty. rewrite it_mkProd_or_LetIn_app /=.
   case: x => [na [body|] ty'] /=; by rewrite IHctx' // /snoc -app_assoc.
 Qed.
+
+Lemma reln_list_lift_above l p Γ :
+  Forall (fun x => exists n, x = tRel n /\ p <= n /\ n < p + length Γ) l ->
+  Forall (fun x => exists n, x = tRel n /\ p <= n /\ n < p + length Γ) (reln l p Γ).
+Proof.
+  generalize (le_refl p).
+  generalize p at 1 3 5.
+  induction Γ in p, l |- *. simpl. auto.
+  intros. destruct a. destruct decl_body. simpl.
+  assert(p0 <= S p) by lia.
+  specialize (IHΓ l (S p) p0 H1). rewrite <- Nat.add_succ_comm, Nat.add_1_r.
+  simpl in *. rewrite <- Nat.add_succ_comm in H0. eauto.
+  simpl in *.
+  specialize (IHΓ (tRel p :: l) (S p) p0 ltac:(lia)). rewrite <- Nat.add_succ_comm, Nat.add_1_r.
+  eapply IHΓ. simpl in *. rewrite <- Nat.add_succ_comm in H0. auto.
+  simpl in *.
+  constructor. exists p. intuition lia. auto.
+Qed.
+
+Lemma to_extended_list_k_spec Γ k :
+  Forall (fun x => exists n, x = tRel n /\ k <= n /\ n < k + length Γ) (to_extended_list_k Γ k).
+Proof.
+  pose (reln_list_lift_above [] k Γ).
+  unfold to_extended_list_k.
+  forward f. constructor. apply f.
+Qed.
+
+Lemma to_extended_list_lift_above Γ :
+  Forall (fun x => exists n, x = tRel n /\ n < length Γ) (to_extended_list Γ).
+Proof.
+  pose (reln_list_lift_above [] 0 Γ).
+  unfold to_extended_list.
+  forward f. constructor. eapply Forall_impl; eauto. intros.
+  destruct H; eexists; intuition eauto.
+Qed.
+
+Fixpoint reln_alt p Γ :=
+  match Γ with
+  | [] => []
+  | {| decl_body := Some _ |} :: Γ => reln_alt (p + 1) Γ
+  | {| decl_body := None |} :: Γ => tRel p :: reln_alt (p + 1) Γ
+  end.
+
+Lemma reln_alt_eq l Γ k : reln l k Γ = List.rev (reln_alt k Γ) ++ l.
+Proof.
+  induction Γ in l, k |- *; simpl; auto.
+  destruct a as [na [body|] ty]; simpl.
+  now rewrite IHΓ.
+  now rewrite IHΓ -app_assoc.
+Qed.
+
+Lemma to_extended_list_k_cons d Γ k :
+  to_extended_list_k (d :: Γ) k =
+  match d.(decl_body) with
+  | None => to_extended_list_k Γ (S k) ++ [tRel k]
+  | Some b => to_extended_list_k Γ (S k)
+  end.
+Proof.
+  rewrite /to_extended_list_k reln_alt_eq. simpl.
+  destruct d as [na [body|] ty]. simpl.
+  now rewrite reln_alt_eq Nat.add_1_r.
+  simpl. rewrite reln_alt_eq.
+  now rewrite -app_assoc !app_nil_r Nat.add_1_r.
+Qed.
+
+Lemma context_assumptions_length_bound Γ : context_assumptions Γ <= #|Γ|.
+Proof.
+  induction Γ; simpl; auto. destruct a as [? [?|] ?]; simpl; auto.
+  lia.
+Qed.
+
+Lemma mapi_rec_compose {A B C} (g : nat -> B -> C) (f : nat -> A -> B) k l :
+  mapi_rec g (mapi_rec f l k) k = mapi_rec (fun k x => g k (f k x)) l k.
+Proof.
+  induction l in k |- *; simpl; auto. now rewrite IHl.
+Qed.
+
+Lemma mapi_compose {A B C} (g : nat -> B -> C) (f : nat -> A -> B) l :
+  mapi g (mapi f l) = mapi (fun k x => g k (f k x)) l.
+Proof. apply mapi_rec_compose. Qed.
+
+Ltac merge_All :=
+  unfold tFixProp, tCaseBrsProp in *;
+  repeat toAll.
 
 Hint Rewrite @map_def_id @map_id : map.
 
@@ -466,6 +550,76 @@ Proof.
 Qed.
 Close Scope string_scope.
 
+Lemma firstn_add {A} x y (args : list A) : firstn (x + y) args = firstn x args ++ firstn y (skipn x args).
+Proof.
+  induction x in y, args |- *. simpl. reflexivity.
+  simpl. destruct args. simpl.
+  now rewrite firstn_nil.
+  rewrite IHx. now rewrite app_comm_cons.
+Qed.
+
+
+Lemma rev_map_spec {A B} (f : A -> B) (l : list A) : 
+  rev_map f l = List.rev (map f l).
+Proof.
+  unfold rev_map.
+  rewrite -(app_nil_r (List.rev (map f l))).
+  generalize (@nil B).
+  induction l; simpl; auto. intros l0.
+  rewrite IHl. now rewrite -app_assoc.
+Qed.
+
+Lemma skipn_0 {A} (l : list A) : skipn 0 l = l.
+Proof. reflexivity. Qed.
+
+Lemma skipn_n_Sn {A} n s (x : A) xs : skipn n s = x :: xs -> skipn (S n) s = xs.
+Proof.
+  induction n in s, x, xs |- *.
+  - unfold skipn. now intros ->.
+  - destruct s; simpl. intros H; discriminate. apply IHn.
+Qed. 
+
+Lemma skipn_all {A} (l : list A) : skipn #|l| l = [].
+Proof.
+  induction l; simpl; auto.
+Qed.
+
+Lemma skipn_app_le {A} n (l l' : list A) : n <= #|l| -> skipn n (l ++ l') = skipn n l ++ l'.
+Proof.
+  induction l in n, l' |- *; simpl; auto.
+  intros Hn. destruct n; try lia. reflexivity.
+  intros Hn. destruct n. reflexivity.
+  rewrite !skipn_S. apply IHl. lia.
+Qed.
+
+Lemma firstn_ge {A} (l : list A) n : #|l| <= n -> firstn n l = l.
+Proof.
+  induction l in n |- *; simpl; intros; auto. now rewrite firstn_nil.
+  destruct n; simpl. lia. rewrite IHl; auto. lia.
+Qed.
+
+Lemma firstn_0 {A} (l : list A) n : n = 0 -> firstn n l = [].
+Proof.
+  intros ->. reflexivity.
+Qed.
+
+
+Arguments firstn : simpl nomatch.
+Arguments skipn : simpl nomatch.
+
+
+Lemma skipn_firstn_skipn {A} (l : list A) n : skipn n (firstn (S n) l) ++ skipn (S n) l = skipn n l.
+Proof.
+  induction l in n |- *; simpl; auto. now rewrite app_nil_r.
+  destruct n=> /=; auto.
+Qed.
+
+Lemma firstn_firstn_firstn {A} (l : list A) n : firstn n (firstn (S n) l) = firstn n l.
+Proof.
+  induction l in n |- *; simpl; auto.
+  destruct n=> /=; auto. now rewrite IHl.
+Qed.
+
 Lemma decompose_app_rec_inv' f l hd args :
   decompose_app_rec f l = (hd, args) ->
   ∑ n, ~~ isApp hd /\ l = skipn n args /\ f = mkApps hd (firstn n args).
@@ -546,3 +700,10 @@ Ltac solve_discr :=
         | [ H : is_true (application_atom (mkApps _ _)) |- _ ] =>
           destruct (application_atom_mkApps H); subst; try discriminate
         end)).
+
+(** Use a coercion for this common projection of the global context. *)
+Definition fst_ctx : global_env_ext -> global_env := fst.
+Coercion fst_ctx : global_env_ext >-> global_env.
+
+Definition empty_ext (Σ : global_env) : global_env_ext
+  := (Σ, Monomorphic_ctx ContextSet.empty).
