pcuic/theories/PCUICSubstitution.v
@@ -2435,3 +2435,99 @@ Proof.
   simpl in thm.
   specialize (thm Ht). now rewrite !subst_empty in thm.
 Qed.
+
+
+Lemma subst_context_comm s s' Γ : 
+  subst_context s 0 (subst_context s' 0 Γ) =
+  subst_context (map (subst s 0) s' ++ s) 0 Γ.
+Proof.
+  intros.
+  rewrite !subst_context_alt !mapi_compose.
+  apply mapi_ext => i x.
+  destruct x as [na [b|] ty] => //.
+  - rewrite /subst_decl /map_decl /=; f_equal.
+    + rewrite !mapi_length. f_equal. rewrite {2}Nat.add_0_r.
+      rewrite subst_app_simpl.
+      rewrite distr_subst_rec. rewrite Nat.add_0_r; f_equal; try lia.
+      rewrite map_length. f_equal; lia.
+    + rewrite mapi_length.
+      rewrite subst_app_simpl.
+      rewrite {2}Nat.add_0_r.
+      rewrite distr_subst_rec. rewrite Nat.add_0_r; f_equal; try lia.
+      rewrite map_length. f_equal; lia.
+  - rewrite /subst_decl /map_decl /=; f_equal.
+    rewrite !mapi_length. rewrite {2}Nat.add_0_r.
+    rewrite subst_app_simpl.
+    rewrite distr_subst_rec. rewrite Nat.add_0_r; f_equal; try lia.
+    rewrite map_length. f_equal. lia.
+Qed.
+
+Lemma substitution_wf_local `{cf : checker_flags} (Σ : global_env_ext) Γ Γ' s Δ :
+  wf Σ -> subslet Σ Γ s Γ' ->
+  wf_local Σ (Γ ,,, Γ' ,,, Δ) ->
+  wf_local Σ (Γ ,,, subst_context s 0 Δ).
+Proof.
+  intros wfΣ subs wfl.
+  induction Δ.
+  { simpl. apply All_local_env_app in wfl as [wfl _].
+    now apply All_local_env_app in wfl as [wfl _]. }
+  destruct a as [na [b|] ty]; depelim wfl; rewrite subst_context_snoc; simpl in *.
+  - constructor.
+    + now apply IHΔ.
+    + simpl in H; noconf H.
+    + simpl in H; noconf H.
+  - simpl in H; noconf H.
+    simpl in *. constructor; auto; red.
+    + simpl. rewrite Nat.add_0_r.
+      destruct l as [s' Hs].
+      eapply substitution in Hs; eauto.
+    + simpl. rewrite Nat.add_0_r.
+      eapply substitution in l0; eauto.
+  - simpl.
+    rewrite /subst_decl. rewrite Nat.add_0_r /map_decl /=.
+    constructor; noconf H; auto.
+    red.
+    destruct l as [s' Hs].
+    exists s'. eapply substitution in Hs; eauto.
+  - constructor; noconf H.
+Qed.
+
+Lemma subst_app_context s s' Γ : subst_context (s ++ s') 0 Γ = subst_context s 0 (subst_context s' #|s| Γ).
+Proof.
+  induction Γ; simpl; auto.
+  rewrite !subst_context_snoc /= /subst_decl /map_decl /=. simpl.
+  rewrite IHΓ. f_equal. f_equal.
+  - destruct a as [na [b|] ty]; simpl; auto.
+    f_equal. rewrite subst_context_length Nat.add_0_r.
+    now rewrite subst_app_simpl.
+  - rewrite subst_context_length Nat.add_0_r.
+    now rewrite subst_app_simpl.
+Qed.
+
+Lemma context_assumptions_subst s n Γ : 
+  context_assumptions (subst_context s n Γ) = context_assumptions Γ.
+Proof. apply context_assumptions_fold. Qed.
+Hint Rewrite context_assumptions_subst : pcuic.
+
+
+Lemma subst_app_simpl' (l l' : list term) (k : nat) (t : term) n :
+  n = #|l| ->
+  subst (l ++ l') k t = subst l k (subst l' (k + n) t).
+Proof. intros ->; apply subst_app_simpl. Qed.
+
+
+Lemma subst_app_context' (s s' : list term) (Γ : context) n :
+  n = #|s| ->  
+  subst_context (s ++ s') 0 Γ = subst_context s 0 (subst_context s' n Γ).
+Proof.
+  intros ->; apply subst_app_context.
+Qed.
+
+
+Lemma map_subst_app_simpl l l' k (ts : list term) : 
+  map (subst l k ∘ subst l' (k + #|l|)) ts =
+  map (subst (l ++ l') k) ts.
+Proof.
+  eapply map_ext. intros.
+  now rewrite subst_app_simpl.
+Qed.
